# [괄호 변환](https://programmers.co.kr/learn/courses/30/lessons/60058)

## Solution 3

```java
class Solution {

    public String solution(String p) {
        if (p.isEmpty()) {
            return "";
        }
        int index = findUIndex(p);
        String u = p.substring(0, index + 1);
        String v = p.substring(index + 1);
        if (u.charAt(0) == '(') {
            v = solution(v);
            return u + v;
        }

        StringBuilder sb = new StringBuilder();
        sb.append('(');
        sb.append(solution(v));
        sb.append(')');
        for (int i = 1; i < u.length() - 1; i++) {
            sb.append(u.charAt(i) == '(' ? ')' : '(');
        }
        return sb.toString();
    }

    private int findUIndex(String p) {
        int index = 0;
        int count = 0;
        while (index < p.length()) {
            count += p.charAt(index) == '(' ? 1 : -1;
            if (count == 0) {
                break;
            }
            index += 1;
        }

        return index;
    }
}
```

## My Solution 2

```java
class Solution {
    public String solution(String p) {
        if (p.isEmpty()) {
            return "";
        }
        int countOpen = 0;
        int countClose = 0;
        int idx = 0;
        boolean correct = true;
        while (idx < p.length()) {
            if (p.charAt(idx) == '(') {
                countOpen += 1;
            } else {
                countClose += 1;
            }

            if (countClose > countOpen) {
                correct = false;
            }

            idx += 1;

            if (countOpen == countClose) {
                break;
            }
        }

        String u = p.substring(0, idx);
        String v = p.substring(idx);

        if (correct) {
            return u + solution(v);
        } else {
            StringBuilder sb = new StringBuilder("(");
            sb.append(solution(v));
            sb.append(")");
            for (int i = 1; i < u.length() - 1; i++) {
                char c = p.charAt(i);
                if (c == '(') {
                    sb.append(')');
                } else {
                    sb.append('(');
                }
            }
            return sb.toString();
        }
    }
}
```

## My Solution 1

```python
def solution(p):
    if not p:
        return ''

    brackets_count = [0, 0]

    for i in range(len(p)):
        if p[i] == '(':
            brackets_count[0] += 1
        else:
            brackets_count[1] += 1

        if brackets_count[0] == brackets_count[1]:
            break

    u, v = p[:i+1], p[i+1:]

    if u[0] == '(':
        v = solution(v)
        return u + v
    else:
        result = "(" + solution(v) + ")"
        for i in range(1, len(u)-1):
            if u[i] == '(':
                result += ')'
            else:
                result += '('

        return result
```

###### 다른 사람 풀이
```python
def solution(p):
    if p=='': return p
    r=True; c=0
    for i in range(len(p)):
        if p[i]=='(': c-=1
        else: c+=1
        if c>0: r=False
        if c==0:
            if r:
                return p[:i+1]+solution(p[i+1:])
            else:
                return '('+solution(p[i+1:])+')'+''.join(list(map(lambda x:'(' if x==')' else ')',p[1:i]) ))
```